lib/pulse/lib/class/Pulse.Class.Droppable.fst
@@ -1,0 +1,43 @@
+(*
+   Copyright 2024 Microsoft Research
+
+   Licensed under the Apache License, Version 2.0 (the "License");
+   you may not use this file except in compliance with the License.
+   You may obtain a copy of the License at
+
+       http://www.apache.org/licenses/LICENSE-2.0
+
+   Unless required by applicable law or agreed to in writing, software
+   distributed under the License is distributed on an "AS IS" BASIS,
+   WITHOUT WARRANTIES OR CONDITIONS OF ANY KIND, either express or implied.
+   See the License for the specific language governing permissions and
+   limitations under the License.
+*)
+
+module Pulse.Class.Droppable
+#lang-pulse
+
+open Pulse.Lib.Core
+module _ = Pulse.Main // required for --ide?
+
+inline_for_extraction fn drop_emp () requires emp ensures emp { () }
+inline_for_extraction instance droppable_emp : droppable emp =
+  { drop_f = drop_emp }
+
+inline_for_extraction fn drop_pure p () requires pure p ensures emp { () }
+inline_for_extraction instance droppable_pure (p: prop) : droppable (pure p) =
+  { drop_f = drop_pure p }
+
+inline_for_extraction fn drop_star (p q: slprop) {| droppable p |} {| droppable q |} ()
+  requires p ** q
+  ensures emp
+{
+  drop p ();
+  drop q ();
+}
+inline_for_extraction instance droppable_star (p q: slprop) {| droppable p |} {| droppable q |} : droppable (p ** q) =
+  { drop_f = drop_star p q }
+
+inline_for_extraction fn drop_inv i p () requires inv i p ensures emp { drop_ (inv i p) }
+inline_for_extraction instance droppable_inv (i : iname) (p : slprop) : droppable (inv i p) =
+  { drop_f = drop_inv i p }
