lib/pulse/lib/class/Pulse.Class.Droppable.fsti
@@ -1,0 +1,33 @@
+(*
+   Copyright 2024 Microsoft Research
+
+   Licensed under the Apache License, Version 2.0 (the "License");
+   you may not use this file except in compliance with the License.
+   You may obtain a copy of the License at
+
+       http://www.apache.org/licenses/LICENSE-2.0
+
+   Unless required by applicable law or agreed to in writing, software
+   distributed under the License is distributed on an "AS IS" BASIS,
+   WITHOUT WARRANTIES OR CONDITIONS OF ANY KIND, either express or implied.
+   See the License for the specific language governing permissions and
+   limitations under the License.
+*)
+
+module Pulse.Class.Droppable
+
+open Pulse.Lib.Core
+
+class droppable (p : slprop) = {
+  drop_f : unit -> stt unit p (fun _ -> emp);
+}
+
+inline_for_extraction
+let drop (p : slprop) {| droppable p |} ()
+  : stt unit p (fun _ -> emp) = drop_f #p ()
+
+inline_for_extraction instance val droppable_emp : droppable emp
+inline_for_extraction instance val droppable_pure (p: prop) : droppable (pure p)
+inline_for_extraction instance val droppable_star (p q: slprop) {| droppable p |} {| droppable q |} : droppable (p ** q)
+
+inline_for_extraction instance val droppable_inv (i : iname) (p : slprop) : droppable (inv i p)
